2 state SIL sound complete

SIL-Parallel/SIL_Sound_Complete.thy
@@ -9,29 +9,16 @@ begin
 subsubsection "Soundness"
 
 lemma sil_while_sound_ok:
-  assumes "\<And>n. \<turnstile> \<langle>Q (Suc n)\<rangle> c  \<langle>OK (Q n)\<rangle>"
+assumes "\<And>n. \<turnstile> \<langle>Q (Suc n)\<rangle> c  \<langle>OK (Q n)\<rangle>"
       and "\<And>s. Q 0 s \<Longrightarrow> \<not> bval b s"
       and "\<And>n s. Q (Suc n) s \<Longrightarrow>  bval b s"
       and "Q n s"
       and "\<And>n. \<forall>s. Q (Suc n) s \<longrightarrow> (\<exists>t. (c, s) \<Down> (t,True) \<and> Q n t)"
     shows "(\<exists>t. (WHILE b DO c, s) \<Down> (t,True) \<and> Q 0 t)"
   using assms
-  apply (induct n arbitrary: s rule: Nat.nat_less_induct, clarsimp)
-    proof -
-        fix na :: nat and sa :: "char list \<Rightarrow> int" and nat :: nat
-        assume a1: "Q na sa"
-        assume a2: "\<forall>m<na. \<forall>x. Q m x \<longrightarrow> (\<exists>t. (WHILE b DO c, x) \<Down> (t, True) \<and> Q 0 t)"
-        obtain ii :: "(char list \<Rightarrow> int) \<Rightarrow> nat \<Rightarrow> char list \<Rightarrow> int" where
-          f3: "\<forall>x0 x1. (\<exists>v2. (c, x0) \<Down> (v2, True) \<and> Q x1 v2) = ((c, x0) \<Down> (ii x0 x1, True) \<and> Q x1 (ii x0 x1))"
-          by moura
-        have f4: "(na < Suc 0) = (na = 0)"
-          by simp
-        have "\<forall>n f. \<not> Q (Suc n) f \<or> (c, f) \<Down> (ii f n, True) \<and> Q n (ii f n)"
-          using f3 assms(5) by presburger
-        then show "\<exists>f. (WHILE b DO c, sa) \<Down> (f, True) \<and> Q 0 f"
-          using f4 a2 a1 by (metis (no_types) Suc_less_eq2 WhileBodySucceeds WhileGuardFalse assms(2,3) lessI nat_neq_iff)
-      qed
-
+  apply (induct n arbitrary: s)
+   apply fastforce
+  by blast
 
 lemma sil_while_sound_er:
   assumes "\<And>n. \<turnstile> \<langle>Q (Suc (Suc n))\<rangle> c \<langle>OK (Q (Suc n))\<rangle>"
@@ -47,6 +34,21 @@ lemma sil_while_sound_er:
   apply fastforce
   apply blast
   done
+
+lemma disjunction_sound:
+  assumes hP: "\<Turnstile> \<langle>P\<rangle> c \<langle>Q\<rangle>"
+      and hR: "\<Turnstile> \<langle>R\<rangle> c \<langle>Q\<rangle>"
+  shows
+    "case Q of
+       OK x \<Rightarrow>
+         \<forall>s. P s \<or> R s \<longrightarrow>
+             (\<exists>t. (c,s) \<Down> (t,True) \<and> x t)
+     | ER x \<Rightarrow>
+         \<forall>s. P s \<or> R s \<longrightarrow>
+             (\<exists>t. (c,s) \<Down> (t,False) \<and> x t)" 
+  apply(cases Q)
+  using SIL_valid_def hP hR apply auto[1]
+using SIL_valid_def hP hR by force
 
 
 lemma sil_sound: 
@@ -73,6 +75,8 @@ lemma sil_sound:
   apply fastforce defer defer
   apply fastforce
   apply fastforce
+     apply (metis (lifting) ext post.case_distrib)
+  apply (simp add: SIL_valid_def disjunction_sound)
   apply clarsimp 
   using sil_while_sound_ok apply auto[1]
   apply clarsimp using sil_while_sound_er by auto
@@ -91,13 +95,39 @@ lemma wp_SKIP_ER [simp]:
   "wp SKIP (ER Q) = (\<lambda>s. False)"
   by (rule ext) (fastforce simp: wp_def)
 
-lemma wp_Ass [simp]: 
-  "wp (x::=a) Q = (\<lambda>s. Q(s[a/x]))"
+lemma wp_ABORT_ER [simp]: 
+  "wp ABORT (ER Q) = Q"
+  by (rule ext) (fastforce simp: wp_def)
+
+lemma wp_ABORT_OK [simp]: 
+  "wp ABORT (OK Q) = (\<lambda>s. False)"
+  by (rule ext) (fastforce simp: wp_def)
+
+lemma wp_Assign_OK [simp]: 
+  "wp (x::=a) (OK Q) = (\<lambda>s. Q(s[a/x]))"
   by (fastforce simp: wp_def)
 
-lemma wp_AssND [simp]: 
-  "wp (x::= ND vals) Q = (\<lambda>s. (\<exists>v \<in> vals. Q (s(x := v))))"
+lemma wp_Assign_ER [simp]: 
+  "wp (x::=a) (ER Q) = (\<lambda>s. False)"
+  using wp_def by fastforce
+
+lemma wp_AssignND_NonEmpty_OK [simp]: 
+  "vals \<noteq> {} \<Longrightarrow> wp (x::= ND vals) (OK Q) = (\<lambda>s. (\<exists>v \<in> vals. Q (s(x := v))))"
   by (fastforce simp: wp_def)
+
+lemma wp_AssignND_NonEmpty_ER [simp]: 
+  "vals \<noteq> {} \<Longrightarrow> wp (x::= ND vals) (ER Q) = (\<lambda>s. False)"
+  by (fastforce simp: wp_def)
+
+lemma wp_AssignND_Empty_ER [simp]: 
+  "vals = {} \<Longrightarrow> wp (x::= ND vals) (ER Q) = Q"
+  unfolding wp_def
+  by auto
+
+lemma wp_AssignND_Empty_OK [simp]: 
+  "vals = {} \<Longrightarrow> wp (x::= ND vals) (OK Q) = (\<lambda>s. False)"
+  unfolding wp_def
+  by auto
 
 lemma wp_SelectND_OK[simp]: 
   "wp (SelectND S) (OK Q) = (\<lambda>s. \<exists>(b,c) \<in> set S. (bval b s) \<and> (wp c (OK Q) s))"
@@ -105,16 +135,15 @@ lemma wp_SelectND_OK[simp]:
 
 lemma wp_SelectND_ER[simp]: 
   "wp (SelectND S) (ER Q) = 
-    (\<lambda>s. (\<exists>(b,c) \<in> set S. (bval b s) \<and> (wp c (ER Q) s)) \<or> (\<forall>(b,c) \<in> set S. \<not>bval b s \<and> Q s))"
+    (\<lambda>s. (\<exists>(b,c) \<in> set S. (bval b s) \<and> (wp c (ER Q) s)) 
+                \<or> ((\<forall>(b,c) \<in> set S. \<not>bval b s) \<and> Q s))"
   apply (rule ext)
   apply (simp add: wp_def)
   apply (rule iffI)
-   apply clarsimp
-   apply blast
-  find_theorems "?P \<or> ?Q \<Longrightarrow> ?R"
-  apply (simp add: imp_disjL)
-  sledgehammer
-Hol
+  apply clarsimp
+  apply blast
+  by blast
+
 lemma wp_Seq_OK[simp]: 
   "wp (c\<^sub>1;;c\<^sub>2) (OK Q) = wp c\<^sub>1 (OK (wp c\<^sub>2 (OK Q)))"
   by (rule ext) (fastforce simp: wp_def)
@@ -135,139 +164,370 @@ lemma wp_While_True[simp]:
   "bval b s \<Longrightarrow> wp (WHILE b DO c) Q s = wp (c;; WHILE b DO c) Q s"
   by(fastforce simp: wp_While_If)
 
-lemma wp_While_False[simp]: 
-  "\<not> bval b s \<Longrightarrow> wp (WHILE b DO c) Q s = Q s"
-  by(fastforce simp: wp_While_If)
+lemma wp_While_False_OK[simp]: 
+  "\<not> bval b s \<Longrightarrow> wp (WHILE b DO c) (OK Q) s  = Q s"
+  by (simp add: wp_While_If)
+
+lemma wp_While_False_ER[simp]: 
+  "\<not> bval b s \<Longrightarrow> wp (WHILE b DO c) (ER Q) s  = False"
+  by (simp add: wp_While_If)
 
 
 subsubsection "Completeness"
+
+thm tSeqOK
+thm tSeqER
+thm SeqE
+thm SeqTrue
+thm SeqFalse
+
+lemma "seq_is_pre":
+  assumes c1: "\<forall>R. \<turnstile> \<langle>wp c1 R\<rangle> c1  \<langle>R\<rangle>"
+  and c2: "\<turnstile> \<langle>wp c2 Q\<rangle> c2  \<langle>Q\<rangle>"
+  shows "\<turnstile> \<langle>wp (c1;; c2) Q\<rangle>
+         c1;; c2 \<langle>Q\<rangle>"
+proof (cases Q)
+  case (OK x)
+  have "\<turnstile> \<langle>wp c1 (OK (wp c2 Q))\<rangle> c1  \<langle>OK (wp c2 Q)\<rangle>"
+    by (metis c1)
+  then show ?thesis
+    using OK c2 by auto
+next
+  case (ER x)
+  have h0: "\<turnstile> \<langle>wp c1 (OK (wp c2 Q))\<rangle> c1  \<langle>OK (wp c2 Q)\<rangle>"
+    by (metis c1)
+  have h1: "\<turnstile> \<langle>wp c1 (OK (wp c2 Q))\<rangle> c1;;c2  \<langle>ER x\<rangle>"
+    by (metis c2 ER h0 tSeqOK)
+  have h2: "\<turnstile> \<langle>wp c1 (ER x)\<rangle> c1  \<langle>ER x\<rangle>"
+    by (metis c1)
+  have h3: "\<turnstile> \<langle>wp c1 (ER x)\<rangle> c1;;c2  \<langle>ER x\<rangle>"
+    by (metis c1 tSeqER)
+  have h4: "\<turnstile> \<langle>\<lambda>s. (wp c1 (ER x)) s \<or> wp c1 (OK (wp c2 Q)) s\<rangle> c1;;c2  \<langle>ER x\<rangle>"
+    by (metis h3 h1 disjunction)
+  then show ?thesis
+    by (smt (verit) ER strengthen_pre wp_Seq_ER)
+qed
+
+
+
+(*(SELECT ?bs, ?s) \<Down> ?t \<Longrightarrow> 
+(\<And>b c. (b, c) \<in> set ?bs \<Longrightarrow> 
+bval b ?s \<Longrightarrow> (c, ?s) \<Down> ?t \<Longrightarrow> ?P) 
+\<Longrightarrow> ?P *)
+
+definition select_pre where
+  "select_pre \<equiv> \<lambda>bs Q. (\<lambda>s.(\<exists>t. (SELECT bs, s) \<Down> t \<and> apply_post Q t))"
+
+definition select_pre_er where
+  "select_pre_er \<equiv> \<lambda>bs Q. wp (SelectND bs) Q"
+
+definition select_path_pre_er where
+  "select_path_pre_er \<equiv> \<lambda>b c Q. (\<lambda>s. (\<exists>t. (c, s) \<Down> (t,False) \<and> post_assn Q t))"
+
+definition select_path_pre_np where
+  "select_path_pre_np  \<equiv> \<lambda>bs Q. (\<lambda>s. \<not>(\<exists>b c. (b,c) \<in> set bs \<and> bval b s) \<and> post_assn Q s)"
+
+definition select_path_pre where
+  "select_path_pre \<equiv> \<lambda>b c Q. (\<lambda>s. (\<exists>t. (c, s) \<Down> t \<and> apply_post Q t))"
+
+lemma SelectND_is_pre:
+  assumes "\<forall>b c. (b,c) \<in> set bs \<longrightarrow> \<turnstile> \<langle>wp c Q\<rangle> c \<langle>Q\<rangle>"
+  shows "\<turnstile> \<langle>wp (SELECT bs) Q\<rangle> SELECT bs \<langle>Q\<rangle>"
+proof(cases Q)
+  case (OK x)
+    have h3: "\<forall>s. select_pre bs Q s \<longrightarrow> 
+        (\<exists>b c. (b,c) \<in> set bs \<and> bval b s \<and> (\<exists>t. (c, s) \<Down> t \<and> apply_post Q t))"
+      by (metis OK SelectNDE apply_post.simps(1) select_pre_def)
+  
+    have h6: "\<forall>bc \<in> set bs. case bc of (b,c) \<Rightarrow> \<turnstile> \<langle>\<lambda>s. select_path_pre b c Q s \<and> bval b s\<rangle> c \<langle>Q\<rangle>"
+      using assms
+      unfolding select_path_pre_def wp_def apply clarsimp
+      by (metis (no_types, lifting) strengthen_pre)
+  
+    hence "\<turnstile> \<langle>select_pre bs Q\<rangle> SELECT bs \<langle>Q\<rangle>" 
+      unfolding select_path_pre_def
+      using h3 by (fastforce intro: tSelectND)
+  
+    thus ?thesis
+      by (fastforce simp: wp_def select_pre_def)
+  next
+    case (ER x)
+    have h3: "\<forall>s. select_pre_er bs Q s \<longrightarrow> (\<exists>(b,c) \<in> set bs. (bval b s) \<and> 
+                (\<exists>t. (c, s) \<Down> t \<and> apply_post Q t)) 
+                \<or> ((\<forall>(b,c) \<in> set bs. \<not>bval b s) \<and> x s)"
+      by (smt (verit, del_insts) ER case_prodE case_prodI select_pre_er_def wp_SelectND_ER wp_def)
+
+    have h4: "\<forall>s. select_pre_er bs Q s \<and> (\<exists>(b,c) \<in> set bs. bval b s) \<longrightarrow> (\<exists>(b,c) \<in> set bs. (bval b s) \<and> 
+                (\<exists>t. (c, s) \<Down> t \<and> apply_post Q t))"
+      using h3 by auto 
+
+    have h4p5: "\<forall>s. select_pre_er bs Q s \<and> \<not> (\<exists>(b,c) \<in> set bs. bval b s) \<longrightarrow> x s"
+      using h3 by auto 
+
+    have h5: "\<forall>s. select_pre_er bs Q s \<and> (\<exists>(b,c) \<in> set bs. bval b s) \<longrightarrow> (\<exists>(b,c) \<in> set bs. (bval b s) \<and> 
+                (\<exists>t. (c, s) \<Down> (t,False) \<and> post_assn Q t))"
+      by (smt (verit, ccfv_threshold) ER apply_post.elims(2) apply_post.simps(2) case_prodE case_prodI h4
+          post_assn.simps(2))
+
+    have h6: "\<forall>bc \<in> set bs. case bc of (b,c) \<Rightarrow>
+       \<turnstile> \<langle>\<lambda>s. (select_path_pre_er b c Q s)  \<and> bval b s\<rangle> c \<langle>Q\<rangle>"
+      using assms
+      unfolding select_path_pre_def wp_def apply clarsimp
+      by (smt (verit) ER apply_post.simps(2) post_assn.simps(2) select_path_pre_er_def
+          strengthen_pre)
+
+    hence "\<turnstile> \<langle>\<lambda>s. (select_pre_er bs Q s \<and> (\<exists>(b,c) \<in> set bs. bval b s))\<rangle> SELECT bs \<langle>Q\<rangle>" 
+      unfolding select_path_pre_er_def
+      using h5 by (fastforce intro: tSelectND)
+
+    have h7: "\<turnstile> \<langle>\<lambda>s. (select_path_pre_np bs Q s)\<rangle> SELECT bs \<langle>Q\<rangle>"
+      by (smt (verit, ccfv_threshold) ER case_prodI2 post_assn.simps(2) select_path_pre_np_def tSelectNDNP
+          weaken_post_er)
+    hence "\<turnstile> \<langle>\<lambda>s. (select_pre_er bs Q s \<and> \<not>(\<exists>(b,c) \<in> set bs. bval b s))\<rangle> SELECT bs \<langle>Q\<rangle>" 
+      unfolding select_path_pre_er_def
+      by (smt (verit) ER case_prod_conv h4p5 post_assn.simps(2) select_path_pre_np_def
+          strengthen_pre)
+
+    have h7p5: "\<turnstile> \<langle>\<lambda>s. (select_pre_er bs Q s \<and> \<not>(\<exists>(b,c) \<in> set bs. bval b s))\<rangle> SELECT bs \<langle>Q\<rangle>"
+      using \<open>\<turnstile> \<langle>\<lambda>s. select_pre_er bs Q s \<and> \<not> (\<exists>(b, c)\<in>set bs. bval b s)\<rangle> SELECT bs \<langle>Q\<rangle>\<close> by blast
+
+    have h6p5: "\<turnstile> \<langle>\<lambda>s. (select_pre_er bs Q s \<and> (\<exists>(b,c) \<in> set bs. bval b s))\<rangle> SELECT bs \<langle>Q\<rangle>"
+      using \<open>\<turnstile> \<langle>\<lambda>s. select_pre_er bs Q s \<and> (\<exists>(b, c)\<in>set bs. bval b s)\<rangle> SELECT bs \<langle>Q\<rangle>\<close> by blast
+
+
+    have h8: "\<turnstile> \<langle>\<lambda>s. (select_pre_er bs Q s \<and> (\<exists>(b,c) \<in> set bs. bval b s)) \<or> (select_pre_er bs Q s \<and> \<not>(\<exists>(b,c) \<in> set bs. bval b s))\<rangle> 
+        SELECT bs \<langle>Q\<rangle>"
+      using disjunction h6p5 h7p5 by blast
+
+    have h9: "\<turnstile> \<langle>select_pre_er bs Q \<rangle> 
+        SELECT bs \<langle>Q\<rangle>"
+      by (metis (no_types, lifting) h8 strengthen_pre)
+
+    thus ?thesis
+      by (metis h9 select_pre_er_def)
+qed
 
 primrec QQ ::
   "(state \<Rightarrow> bool) \<Rightarrow> bexp \<Rightarrow> com \<Rightarrow> nat \<Rightarrow> state \<Rightarrow> bool"
 where
   "QQ R b c 0 = (\<lambda>s. R s \<and> \<not> bval b s)"
-| "QQ R b c (Suc n) = (\<lambda>s. wp c (QQ R b c n) s \<and> bval b s)"
+| "QQ R b c (Suc n) = (\<lambda>s. wp c (OK (QQ R b c n)) s \<and> bval b s)"
+
+primrec QQ_er_1 ::
+  "(state \<Rightarrow> bool) \<Rightarrow> bexp \<Rightarrow> com \<Rightarrow> nat \<Rightarrow> state \<Rightarrow> bool"
+  where
+  "QQ_er_1 R b c 0 = (\<lambda>s. wp c (ER R) s \<and> bval b s)"
+| "QQ_er_1 R b c (Suc n) = (\<lambda>s. wp c (OK (QQ_er_1 R b c n)) s \<and> bval b s)"
+
+primrec QQ_er ::
+  "(state \<Rightarrow> bool) \<Rightarrow> bexp \<Rightarrow> com \<Rightarrow> nat \<Rightarrow> state \<Rightarrow> bool"
+  where
+  "QQ_er R b c 0 = R"
+| "QQ_er R b c (Suc n) = QQ_er_1 R b c n"
 
 
 lemma While_Strengthen:
   assumes exec: "(WHILE b DO c, s) \<Down> t"
-  and post: "Q t"
+  and post: "apply_post (OK Q) t"
   shows "\<exists>n. (QQ Q b c) n  s"
   using exec post
 proof (induction "(WHILE b DO c, s)" t arbitrary: Q s rule: big_step.induct)
-  case  WhileFalse then show ?case
-    by (meson QQ.simps(1))
-    next 
-      case (WhileTrue s1 s2 s3) 
+  case  WhileGuardFalse then show ?case
+    by (meson QQ.simps(1) apply_post.simps(1))
+  next 
+  case (WhileBodySucceeds s1 s2 s3) 
       then obtain n where hn: "QQ Q b c n s2"
-        using WhileTrue.hyps(2) WhileTrue.prems
-        by presburger
+        by blast
       then have h0: "QQ Q b c n s2"
         by simp
-      then have h1: "wp c (QQ Q b c n) s1"
+      then have h1: "wp c (OK (QQ Q b c n)) s1"
         unfolding wp_def
       proof-
-        show "\<exists>t. (c, s1) \<Down> t \<and> QQ Q b c n t"
-        proof (rule exI[where x=s2])
-          show "(c, s1) \<Down> s2 \<and> QQ Q b c n s2"
-          using assms
-          by (simp add: WhileTrue.hyps(2) hn)
+        show "\<exists>t. (c, s1) \<Down> t \<and> apply_post (OK (QQ Q b c n)) t"
+          using WhileBodySucceeds.hyps(2) hn by auto
       qed
-    qed
-    then have h2: "wp c (QQ Q b c n) s1 \<and> bval b s1"
-      by (metis h1 WhileTrue.hyps(1))      
+    then have h2: "wp c (OK (QQ Q b c n)) s1 \<and> bval b s1"
+      by (metis h1 WhileBodySucceeds.hyps(1))    
     show "\<exists>n. QQ Q b c n s1"
         proof (rule exI[where x="Suc n"])
           show "QQ Q b c (Suc n) s1"
             by (simp add: h2)
         qed
-    qed
-        
+   next
+     case (WhileBodyAborts s1 s2)
+     then obtain n where hn: "QQ Q b c n s2"
+       by force
+      then have h0: "QQ Q b c n s2"
+        by simp
+      then have h1: "wp c (ER (QQ Q b c n)) s1"
+        unfolding wp_def
+      proof-
+        show "\<exists>t. (c, s1) \<Down> t \<and> apply_post (ER (QQ Q b c n)) t"
+          using WhileBodyAborts.prems by auto
+      qed
+    then have h2: "wp c (ER (QQ Q b c n)) s1 \<and> bval b s1"
+      by (metis h1 WhileBodyAborts.hyps(1))
+    show "\<exists>n. QQ Q b c n s1"
+        proof (rule exI[where x="Suc n"])
+            show "QQ Q b c (Suc n) s1"
+              using WhileBodyAborts.prems by auto
+          qed
+qed
 
-lemma While_is_pre:
-  assumes "(\<forall>Q. \<turnstile> \<langle>wp c Q\<rangle> c  \<langle>Q\<rangle>)"
-  shows "\<turnstile> \<langle>wp (WHILE b DO c) Q\<rangle> (WHILE b DO c) \<langle>Q\<rangle>"
+lemma While_Strengthen_ER:
+  assumes exec: "(WHILE b DO c, s) \<Down> t"
+  and post: "apply_post (ER Q) t"
+  shows "\<exists>n. (QQ_er Q b c) (Suc n) s"
+  using exec post
+  apply (induction "(WHILE b DO c, s)" t arbitrary: Q s rule: big_step.induct)
+    apply simp
+   defer
+   apply clarsimp
+   apply (metis QQ_er_1.simps(1) apply_post.simps(2) wp_def)
+  apply clarsimp
+proof-
+  fix s\<^sub>1 s\<^sub>2 a Q
+  assume bval: "bval b s\<^sub>1"
+     and c_step: "(c, s\<^sub>1) \<Down> (s\<^sub>2, True)"
+     and while_step: "(WHILE b DO c, s\<^sub>2) \<Down> (a, False)"
+     and IH: "\<And>Q. Q a \<Longrightarrow> \<exists>n. QQ_er_1 Q b c n s\<^sub>2"
+     and Qa: "Q a"
+
+  obtain n where hn: "QQ_er_1 Q b c n s\<^sub>2"
+    by (metis Qa IH)
+  then have h0: "QQ_er_1 Q b c n s\<^sub>2"
+    by simp
+  then have h1: "wp c (OK (QQ_er_1 Q b c n)) s\<^sub>1"
+    unfolding wp_def
+    using c_step by auto
+  then have h2: "wp c (OK (QQ_er_1 Q b c n)) s\<^sub>1 \<and> bval b s\<^sub>1"
+    by (metis h1 bval)
+  show "\<exists>n. QQ_er_1 Q b c n s\<^sub>1"
+    by (meson QQ_er_1.simps(2) h2)
+qed
+
+lemma While_is_pre_ok:
+  assumes "\<forall>Q. \<turnstile> \<langle>wp c (OK Q)\<rangle> c  \<langle>OK Q\<rangle>"
+  shows "\<turnstile> \<langle>wp (WHILE b DO c) (OK Q)\<rangle> (WHILE b DO c) \<langle>(OK Q)\<rangle>"
   unfolding wp_def  
 proof- 
   fix n
-  have h1: "\<turnstile> \<langle>wp c (QQ Q b c n)\<rangle> c  \<langle>QQ Q b c n\<rangle>"
+  have h1: "\<turnstile> \<langle>wp c (OK (QQ Q b c n))\<rangle> c  \<langle>OK (QQ Q b c n)\<rangle>"
     by (metis assms)
-  have h2: "\<turnstile> \<langle>\<lambda>s. (wp c (QQ Q b c n) s \<and> bval b s)\<rangle> c  \<langle>QQ Q b c n\<rangle>"
-    by (smt (verit, ccfv_SIG) conseq h1)
-  have h3: "\<turnstile> \<langle>(QQ Q b c (Suc n))\<rangle> c  \<langle>QQ Q b c n\<rangle>"
+  have h2: "\<turnstile> \<langle>\<lambda>s. (wp c (OK (QQ Q b c n)) s \<and> bval b s)\<rangle> c  \<langle>OK (QQ Q b c n)\<rangle>"
+    by (smt (verit, best) conseqOK h1)
+  have h3: "\<turnstile> \<langle>(QQ Q b c (Suc n))\<rangle> c  \<langle>OK (QQ Q b c n)\<rangle>"
     by (simp add: h2)
-  have h4: "\<And>n::nat. \<turnstile> \<langle>(QQ Q b c) (Suc n)\<rangle> c  \<langle>(QQ  Q b c) n\<rangle>"
+  have h4: "\<And>n::nat. \<turnstile> \<langle>(QQ Q b c) (Suc n)\<rangle> c  \<langle>OK ((QQ  Q b c) n)\<rangle>"
     by (metis QQ.simps(2) assms strengthen_pre)
   have h5: "\<And>s. (QQ Q b c) 0 s \<Longrightarrow> \<not> bval b s"
     by simp
   have h6: "\<And>n s. (QQ Q b c) (Suc n) s \<Longrightarrow> bval b s"
     by simp
-  have h7: "\<turnstile> \<langle>\<lambda>s. \<exists>n. (QQ Q b c) n  s\<rangle> WHILE b DO c \<langle>\<lambda>s. (QQ Q b c) 0 s\<rangle>"
+  have h7: "\<turnstile> \<langle>\<lambda>s. \<exists>n. (QQ Q b c) n  s\<rangle> WHILE b DO c \<langle>OK (\<lambda>s. (QQ Q b c) 0 s)\<rangle>"
     using QQ_def
-    by (smt (verit, best) conseq h4 h5 h6 tWhile)
-  have h8: "\<turnstile> \<langle>\<lambda>s. \<exists>n. (QQ Q b c) n  s\<rangle> WHILE b DO c \<langle>Q\<rangle>"
-    using QQ.simps(1) h7 weaken_post by presburger
-  have h9: "\<turnstile> \<langle>\<lambda>s. \<exists>t. (WHILE b DO c, s) \<Down> t \<and> Q t\<rangle> WHILE b DO c \<langle>Q\<rangle>"
-    by (smt (verit, best) While_Strengthen conseq h8)
-  show "\<turnstile> \<langle>\<lambda>s. \<exists>t. (WHILE b DO c, s) \<Down> t \<and> Q t\<rangle> WHILE b DO c \<langle>Q\<rangle>"
+    by (smt (verit, best) conseqOK h4 h5 h6 tWhileOK)
+  have h8: "\<turnstile> \<langle>\<lambda>s. \<exists>n. (QQ Q b c) n  s\<rangle> WHILE b DO c \<langle>OK Q\<rangle>"
+    using QQ.simps(1) h7 weaken_post_ok by presburger
+  have h9: "\<turnstile> \<langle>\<lambda>s. \<exists>t. (WHILE b DO c, s) \<Down> t \<and> apply_post (OK Q) t\<rangle> WHILE b DO c \<langle>OK Q\<rangle>"
+    by (smt (verit, best) While_Strengthen conseqOK h8)
+  show "\<turnstile> \<langle>\<lambda>s. \<exists>t. (WHILE b DO c, s) \<Down> t \<and> apply_post (OK Q) t\<rangle> WHILE b DO c \<langle>OK Q\<rangle>"
     by (metis h9)
 qed
 
-
-lemma AssignND_is_pre: 
-  "\<turnstile> \<langle>wp (x ::= ND vals) Q\<rangle> x ::= ND vals  \<langle>Q\<rangle>"
-  using wp_AssND 
-  by (fastforce simp: wp_def tAssignND)
-
-definition select_pre where
-  "select_pre \<equiv> \<lambda>bs Q. (\<lambda>s.(\<exists>t. (SELECT bs, s) \<Down> t \<and> Q t))"
-
-definition select_path_pre where
-  "select_path_pre \<equiv> \<lambda>b c Q. (\<lambda>s. (\<exists>t. (c, s) \<Down> t \<and> Q t))"
-
-lemma SelectND_is_pre:
-  assumes "\<forall>b c. (b,c) \<in> set bs \<longrightarrow> \<turnstile> \<langle>wp c Q\<rangle> c \<langle>Q\<rangle>"
-    shows "\<turnstile> \<langle>wp (SELECT bs) Q\<rangle> SELECT bs \<langle>Q\<rangle>"
+lemma While_is_pre_er:
+  assumes "\<forall>Q. \<turnstile> \<langle>wp c Q\<rangle> c  \<langle>Q\<rangle>"
+  shows "\<turnstile> \<langle>wp (WHILE b DO c) (ER Q)\<rangle> (WHILE b DO c) \<langle>(ER Q)\<rangle>"
+  unfolding wp_def
+  apply clarsimp 
 proof-
-  have h3: "\<forall>s. select_pre bs Q s \<longrightarrow> (\<exists>b c. (b,c) \<in> set bs \<and> bval b s \<and> (\<exists>t. (c, s) \<Down> t \<and> Q t))"
-    unfolding select_pre_def by blast
-
-  have h6: "\<forall>bc \<in> set bs. case bc of (b,c) \<Rightarrow> \<turnstile> \<langle>\<lambda>s. select_path_pre b c Q s \<and> bval b s\<rangle> c \<langle>Q\<rangle>"
-    using assms
-    unfolding select_path_pre_def wp_def apply clarsimp
-    by (metis (no_types, lifting) strengthen_pre)
-
-  hence "\<turnstile> \<langle>select_pre bs Q\<rangle> SELECT bs \<langle>Q\<rangle>" 
-    unfolding select_path_pre_def
-    using h3 by (fastforce intro: tSelectND)
-
-  thus ?thesis
-    by (fastforce simp: wp_def select_pre_def)
+  have h0: "\<exists>a ba. (WHILE b DO c, s) \<Down> (a, ba) \<and> Q a \<and> \<not> ba 
+              \<longleftrightarrow> 
+            (\<exists>a. (WHILE b DO c, s) \<Down> (a, False) \<and> Q a)"
+    by blast
+  fix n
+  have h0: "\<turnstile> \<langle>wp c (ER (QQ_er Q b c 0))\<rangle> c  \<langle>ER (QQ_er Q b c 0)\<rangle>"
+    by (metis assms)
+  have h1: "\<turnstile> \<langle>wp c (OK (QQ_er Q b c (Suc n)))\<rangle> c  \<langle>OK (QQ_er Q b c (Suc n))\<rangle>"
+    by (metis assms)
+  have h2: "\<turnstile> \<langle>\<lambda>s. (wp c (OK (QQ_er Q b c (Suc n))) s \<and> bval b s)\<rangle> c  \<langle>OK (QQ_er Q b c (Suc n))\<rangle>"
+    by (metis (no_types, lifting) assms strengthen_pre_ok)
+  have h3: "\<turnstile> \<langle>(QQ_er Q b c (Suc (Suc n)))\<rangle> c  \<langle>OK (QQ_er Q b c (Suc n))\<rangle>"
+    using h2 by auto
+  have h4: "\<And>n::nat. \<turnstile> \<langle>(QQ_er Q b c) (Suc (Suc n))\<rangle> c  \<langle>OK ((QQ_er Q b c) (Suc n))\<rangle>"
+    by (metis QQ_er.simps(2) QQ_er_1.simps(2) assms strengthen_pre_ok)
+  have h5: "\<turnstile> \<langle>QQ_er Q b c 1\<rangle> c  \<langle>ER (QQ_er Q b c 0)\<rangle>"
+    by (metis One_nat_def QQ_er.simps(1,2) QQ_er_1.simps(1) assms strengthen_pre_er)
+  have h6: "\<And>n s. (QQ_er Q b c) (Suc n) s \<Longrightarrow> bval b s"
+    by (metis QQ_er.simps(2) QQ_er_1.simps(1,2) old.nat.exhaust)
+  have h7: "\<turnstile> \<langle>\<lambda>s. \<exists>n. (QQ_er Q b c) (Suc n)  s\<rangle> WHILE b DO c \<langle>ER (\<lambda>s. (QQ_er Q b c) 0 s)\<rangle>"
+    using h4 h5 h6 tWhileER by blast
+  have h8: "\<turnstile> \<langle>\<lambda>s. \<exists>n. (QQ_er Q b c) (Suc n)  s\<rangle> WHILE b DO c \<langle>ER Q\<rangle>"
+    using h7 by auto
+  have h9: "\<turnstile> \<langle>\<lambda>s. \<exists>t. (WHILE b DO c, s) \<Down> (t,False) \<and> Q t\<rangle> WHILE b DO c \<langle>ER Q\<rangle>"
+    by (smt (verit, ccfv_threshold) While_Strengthen_ER apply_post.simps(2) h8 strengthen_pre)
+  show "\<turnstile> \<langle>\<lambda>s. \<exists>a ba. (WHILE b DO c, s) \<Down> (a, ba) \<and> Q a \<and> \<not> ba\<rangle>
+            WHILE b DO c  
+          \<langle>ER Q\<rangle> " 
+    by (smt (verit, ccfv_SIG) conseqER h9)
 qed
+
 
 lemma wp_is_pre: "\<turnstile> \<langle>wp c Q\<rangle> c \<langle>Q\<rangle>"
   proof(induction c arbitrary: Q)
-    case If thus ?case by(force intro: conseq)
+    case SKIP
+    then show ?case
+      by (metis false_pre post_assn.elims strengthen_pre tSkip wp_SKIP_ER wp_SKIP_OK)
+    case ABORT
+    then show ?case
+      by (metis false_pre post_assn.elims strengthen_pre tAbort wp_ABORT_ER wp_ABORT_OK)
   next
-    case SKIP thus ?case by force
+    case (Assign x1 x2)
+    then show ?case 
+      apply (cases Q)
+      apply simp
+    by (metis wp_Assign_ER strengthen_pre_er false_pre)
   next
-    case Assign thus ?case  by force
+    case (AssignND x1 x2)
+    then show ?case 
+      apply (cases Q)
+      apply clarsimp
+      apply (smt (verit, best) strengthen_pre_ok tAssignNDOK wp_AssignND_Empty_OK
+          wp_AssignND_NonEmpty_OK)
+      by (metis false_pre wp_AssignND_Empty_ER wp_AssignND_NonEmpty_ER strengthen_pre tAssignNDER)
   next
-    case Seq thus ?case by force
+    case (Seq c1 c2)
+    then show ?case
+      by (meson seq_is_pre)
   next
-    case AssignND thus ?case by (rule AssignND_is_pre)
+    case (If x1 c1 c2)
+    then show ?case
+      by (smt (verit, best) strengthen_pre tIf wp_If)
   next
-    case SelectND thus ?case 
-      using SelectND_is_pre by force
+    case (SelectND x)
+    then show ?case
+      by (simp add: SelectND_is_pre)
   next
-    case While thus ?case using While_is_pre by force
-  qed
+    case (While x1 c)
+    then show ?case
+      apply (cases Q)
+      apply clarsimp
+      apply (metis While_is_pre_ok)
+    by (metis While_is_pre_er)
+qed
 
+lemma valid_imp_wp: "\<Turnstile> \<langle>P\<rangle> c  \<langle>Q\<rangle> \<Longrightarrow>
+    \<forall>s. P s \<longrightarrow> wp c Q s"
+  unfolding wp_def SIL_valid_def
+  apply(cases Q)
+  apply fastforce
+by fastforce
 
 lemma sil_complete: 
   "\<Turnstile> \<langle>P\<rangle> c \<langle>Q\<rangle> \<Longrightarrow> \<turnstile> \<langle>P\<rangle> c \<langle>Q\<rangle>"
   apply (rule strengthen_pre[where P="wp c Q"])
-  by (fastforce intro: wp_is_pre simp: SIL_valid_def wp_def)+
+  apply (metis valid_imp_wp)
+by (metis wp_is_pre)
 
 corollary sil_sound_complete: 
   "\<turnstile> \<langle>P\<rangle>c\<langle>Q\<rangle> \<longleftrightarrow> \<Turnstile> \<langle>P\<rangle>c\<langle>Q\<rangle>"
